* Solution

  字符串 =babad=
  |   | j | 0 | 1 | 2 | 3 | 4 |
  | i | @ | b | a | b | a | d |
  |---+---+---+---+---+---+---|
  | 0 | b | 1 | 0 | 1 | 0 | 0 |
  | 1 | a |   | 1 | 0 | 1 | 0 |
  | 2 | b |   |   | 1 | 0 | 0 |
  | 3 | a |   |   |   | 1 | 0 |
  | 4 | d |   |   |   |   | 1 |
  
  * i <= j
  * 当 i == j, table[i][j]=true
  * 当 str[i] == str[j] and table[i+1][j-1]

    1. 计算 i - j == 0
       |   | j | 0 | 1 | 2 | 3 | 4 |
       | i | @ | b | a | b | a | d |
       |---+---+---+---+---+---+---|
       | 0 | b | 1 |   |   |   |   |
       | 1 | a |   | 1 |   |   |   |
       | 2 | b |   |   | 1 |   |   |
       | 3 | a |   |   |   | 1 |   |
       | 4 | d |   |   |   |   | 1 |
    2. 计算 j - i == 1
       |   | j | 0 | 1 | 2 | 3 | 4 |
       | i | @ | b | a | b | a | d |
       |---+---+---+---+---+---+---|
       | 0 | b | 1 | 0 |   |   |   |
       | 1 | a |   | 1 | 0 |   |   |
       | 2 | b |   |   | 1 | 0 |   |
       | 3 | a |   |   |   | 1 | 0 |
       | 4 | d |   |   |   |   | 1 |
    3. 计算 j - i == 2
       |   | j | 0 | 1 | 2 | 3 | 4 |
       | i | @ | b | a | b | a | d |
       |---+---+---+---+---+---+---|
       | 0 | b | 1 | 0 | 1 |   |   |
       | 1 | a |   | 1 | 0 | 1 |   |
       | 2 | b |   |   | 1 | 0 | 0 |
       | 3 | a |   |   |   | 1 | 0 |
       | 4 | d |   |   |   |   | 1 |
    4. 计算 j - i == 3
       |   | j | 0 | 1 | 2 | 3 | 4 |
       | i | @ | b | a | b | a | d |
       |---+---+---+---+---+---+---|
       | 0 | b | 1 | 0 | 1 | 0 |   |
       | 1 | a |   | 1 | 0 | 1 | 0 |
       | 2 | b |   |   | 1 | 0 | 0 |
       | 3 | a |   |   |   | 1 | 0 |
       | 4 | d |   |   |   |   | 1 |
    5. 计算 j - i == 4
       |   | j | 0 | 1 | 2 | 3 | 4 |
       | i | @ | b | a | b | a | d |
       |---+---+---+---+---+---+---|
       | 0 | b | 1 | 0 | 1 | 0 | 0 |
       | 1 | a |   | 1 | 0 | 1 | 0 |
       | 2 | b |   |   | 1 | 0 | 0 |
       | 3 | a |   |   |   | 1 | 0 |
       | 4 | d |   |   |   |   | 1 |

** 空间使用优化
   (i, j) ==> i * len + j
   优化，抠掉下半部分，空白的长度：
   i * len + i - i * (i + 1) / 2
